\documentclass{article}

\usepackage{amsmath}

\begin{document}
\section{Gradient Descent}

\begin{align}
  C'(w) = \lim_{\epsilon \to 0} \frac{C(w + \epsilon) - C(w_i)}{\epsilon}
\end{align}

\subsection{``Twice''}

\begin{align}
  C(w) &= \frac{1}{n}\sum_{i=1}^{n}(x_iw - y_i)^2\\
  C'(w) &= \left(\frac{1}{n}\sum_{i=1}^{n}(x_iw - y_i)^2\right)'\\
       &= \frac{1}{n} \left(\sum_{i=1}^{n}(x_iw - y_i)^2\right)'\\
       &= \frac{1}{n}\sum_{i=1}^{n} \left((x_iw - y_i)^2\right)'\\
       &= \frac{1}{n}\sum_{i=1}^{n}2(x_iw - y_i)\left(x_iw - y_i\right)'\\
       &= \frac{1}{n}\sum_{i=1}^{n}2(x_iw - y_i)x_i
\end{align}

\subsection{One Neuron Model with 2 inputs - sigmoid}

\begin{align}
  y &= \sigma(xw + b) \\
  \sigma(x) &= \frac{1}{1 + e^{-x}} \\
  \sigma'(x) &= \sigma(x)(1 -  \sigma(x))
\end{align}

\subsection{Cost}

\begin{align}
  a_i &= \sigma(wx + b) \\
  C &= \frac{1}{n} \sum_{i=0}^{n}(a_i - z_i)^2 \\
  \partial_{w1}C &= \partial_w\left(\frac{1}{n} \sum_{i=0}^{n}(a_i-z_i)^2 \right) \\
      &= \frac{1}{n} \sum_{i=0}^{n}2(a_i-z_i)\partial_{w1}a_i \\
      &= \frac{1}{n} \sum_{i=0}^{n}2(a_i-z_i)a_i(1-a_i)x_i \\
  \partial_{w2}C&= \frac{1}{n} \sum_{i=0}^{n}2(a_i-z_i)a_i(1-a_i)y_i \\
  \partial_bC &= \frac{1}{n} \sum_{i=0}^{n}2(a_i-z_i)a_i(1-a_i)
\end{align}

\subsection{Two Neuron Model with 1 input}

\begin{align}
  a_i^{(1)} &= \sigma(x_i w^{(1)} + b^{(1)}) \\  
  a^{(1)} &= \sigma(xw^{(1)} + b^{(1)}) \\
  a^{(2)} &= \sigma(a^{(1)}w^{(2)} + b^{(2)}) \\
  \partial_{w^{(2)}}a_i^{(2)} &= a_i^{(2)}(1-a_i^{(2)})a_i^{(1)} \\  
  \partial_{b^{(2)}}a_i^{(2)} &= a_i^{(2)}(1-a_i^{(2)}) \\
  \partial_{a_i^{(1)}}a_i^{(2)} &= a_i^{(2)}(1-a_i^{(2)})w^{(2)}
\end{align}

\subsection{Back-Propagation}
\begin{align}
  C^{(2)} &= \frac{1}{n}\sum_{i=1}^{n}(a_i^{(2)} - y_i)^2 \\
  \partial_{w^{(2)}}C^{(2)} &= \frac{1}{n}\sum_{i=1}^{n} \partial_{w^{(2)}} ((a_i^{(2)} - y_i)^2) \\
            &= \frac{1}{n}\sum_{i=1}^{n}2(a_i^{(2)}-y_i)\partial_{w^{(2)}}a_i^{(2)} \\
            &= \frac{1}{n}\sum_{i=1}^{n}2(a_i^{(2)}-y_i)a_i^{(2)}(1-a_i^{(2)})a_i^{(1)} \\
  \partial_{b^{(2)}}C^{(2)} &= \frac{1}{n}\sum_{i=1}^{n}2(a_i^{(2)}-y_i)a_i^{(2)}(1-a_i^{(2)}) \\
  \partial_{a^{(1)}}C^{(2)} &= \frac{1}{n}\sum_{i=1}^{n}2(a_i^{(2)}-y_i)a_i^{(2)}(1-a_i^{(2)})w^{(2)} \\
  e_i &= a_i^{(1)} - (a_i^{(1)} - \partial_{a^{(1)}}C^{(2)}) \\
  C^{(1)} &= \frac{1}{n}\sum_{i=1}^{n}(a_i^{(1)} - e_i)^2 \\
  \partial_{w^{(1)}}C^{(1)} &= \partial_{w^{(1)}}\left(\frac{1}{n}\sum_{i=1}^{n}  (a_i^{(1)} - e_i)^2\right) \\
          &= \frac{1}{n}\sum_{i=1}^{n} \partial_{w^{(1)}}\left((a_i^{(1)} - e_i)^2\right) \\
            &= \frac{1}{n}\sum_{i=1}^{n} 2(a_i^{(1)} - e_i) \partial_{w^{(1)}}a_i^{(i)}\\
            &= \frac{1}{n}\sum_{i=1}^{n} 2(\partial_{a^{(1)}}C^{(2)})x_i \\  
  \partial_{b^{(1)}}C^{(1)} &= \frac{1}{n}\sum_{i=1}^{n} 2(\partial_{a^{(1)}}C^{(2)})x_i
\end{align}

\end{document}
